\begin{enumerate}[label=(\Alph*)]
    \item $m, m + 3$
    \item $-m, m + 3$
    \item $m, -(m + 3)$
    \item $-m, -(m + 3)$
\end{enumerate}
\item The roots of the equation $x^3 - 3x - \brak{m(m + 3)} = 0$, where $m$ is a constant, are:

\begin{enumerate}[label=(\Alph*)]
    \item $m, m + 3$
    \item $-m, m + 3$
    \item $m, -(m + 3)$
    \item $-m, -(m + 3)$
\end{enumerate}

\item Find the value of $m$ so that the quadratic equation $mx^2 = 6t + (L - x)$ has two equal roots.     
     
\item Find the roots of the following quadratic equation: $x^2 - 3\sqrt{5} \cdot x + 10 = 0$. 

\item Find the roots of the equation $\dfrac{1}{2x-3} + \dfrac{1}{x-5} = 1$, where $x \neq \dfrac{3}{2}, 5$.
\end{enumerate}
