\solution 
\begin{enumerate}
\item From 
	\eqref{eq:median-e}
	and
	\eqref{eq:median-g},
\begin{align}
		\label{eq:tri-pts/4} \vec{G}-\vec{B} &= \myvec{2 \\ -6},\, 
 \vec{E}-\vec{G} = \myvec{1 \\ -3} \\
	\implies \vec{G}-\vec{B} &= 2 \brak{ \vec{E}-\vec{G} }
	\\
	\implies \norm{\vec{G}-\vec{B}} &= 2 \norm{ \vec{E}-\vec{G} }
	\\
	\text{or, }		\label{eq:tri-pts/8}\frac{BG}{GE} &=  2  
\end{align}		
\item From 
	\eqref{eq:median-f}
	and
	\eqref{eq:median-g},
\begin{align}
		 \vec{F}-\vec{G} &= \frac{1}{2}\myvec{ 1 \\ 5},\, 
 \vec{G}-\vec{C} &= \myvec{1 \\ 5} \\
	\implies 		 \vec{G}-\vec{C} &= 2 \brak{\vec{F}-\vec{G}} 
	\\
	\implies 		 \norm{\vec{G}-\vec{C}} &= 2 \norm{\vec{F}-\vec{G}} 
	\\
		\text{or, }	\frac{CG}{GF} &=  2		
\label{eq:tri-pts/9}
\end{align}
\item From
	\eqref{eq:median-d}
	and
	\eqref{eq:median-g},
\begin{align}
		\label{eq:tri-pts/14} \vec{G}-\vec{A} &= \myvec{-3 \\ 1} ,\,
 \vec{D}-\vec{G} = \frac{1}{2}\myvec{ -3 \\ 1}
 \\
	\vec{G}-\vec{A} &= 
	2\brak{ \vec{D}-\vec{G} } 
	\\
\implies		 \norm{\vec{G}-\vec{A}} &= 
 2\norm{\vec{D}-\vec{G}} 
 \\
		\text{or, }		\label{eq:tri-pts/18}\frac{AG}{GD} &=   2		
\end{align}
\end{enumerate}
From \eqref{eq:tri-pts/8}, \eqref{eq:tri-pts/9}, \eqref{eq:tri-pts/18}
\begin{align}
		\frac{BG}{GE} = 
		\frac{CG}{GF} =
		\frac{AG}{GD} = 2
\end{align}
