\solution
Given, 
\begin{align}
\vec{A} = \myvec{1\\-1},
\vec{B} = \myvec{-4\\6},
\vec{C} = \myvec{-3\\-5} \\  
a =  \norm{\vec{B}-\vec{C}}\ &=  \sqrt{\brak{\vec{B}-\vec{C}}^{\top}\brak{\vec{B}-\vec{C}}} \\
 \vec{B}-\vec{C} &= \myvec{-4 \\ 6} - \myvec{-3 \\ -5} \\
 \vec{B}-\vec{C} &= \myvec{-1 \\ 11} \\
 \brak{\vec{B}-\vec{C}}^{\top} &= {\myvec{-1 \\ 11}}^{\top} = \myvec{-1 \ 11} \\
\brak{\vec{B}-\vec{C}}^{\top}\brak{\vec{B}-\vec{C}} &= \myvec{-1 \ 11} \myvec{-1 \\ 11}\\
             &= 1+121 \\
             &= 122 \\  
 \sqrt{\brak{\vec{B}-\vec{C}}^{\top}\brak{\vec{B}-\vec{C}}} &= \sqrt{122}	\\
\implies \norm{\vec{B}-\vec{C}}\ &= \sqrt{122} 
\end{align}
