Find the principal values of the following
\begin{enumerate}[label=\thesubsection.\arabic*,ref=\thesubsection.\theenumi,itemsep=1ex]
\begin{multicols}{4}
\item $\sin ^{-1}\brak{\frac{1}{\sqrt{2}}}$.
\item 	$\cot^{-1}-\brak{\frac{1}{\sqrt{3}}}$.
\item $\sin^{-1}-\brak{\frac{1}{2}}$.
\item $\cos^{-1}\brak{\frac{\sqrt{3}}{2}}$.
	\item $\csc^{-1}{2}$.
	\item $\tan^{-1}\brak{-\sqrt{3}}$.
	\item $\cos^{-1}\brak{-\frac{1}{2}}$.
	\item $\tan^{-1}\brak{-1}$.
	\item $\sec^{-1}\brak{\frac{2}{\sqrt{3}}}$.
	\item $\cot^{-1}\sqrt{3}$.
	\item $\cos^{-1}\brak{-\frac{1}{\sqrt{2}}}$.
	\item $\csc^{-1}\brak{-\sqrt{2}}$.
\end{multicols}
\end{enumerate}
Find the values of the following
\begin{enumerate}[label=\thesubsection.\arabic*,ref=\thesubsection.\theenumi,resume*,itemsep=1ex]
	\item $\tan^{-1}1+\cos^{-1}\brak{-\frac{1}{2}}+\sin^{-1}\brak{-\frac{1}{2}}$
	\item $\cos^{-1}\brak{\frac{1}{2}}+2\sin^{-1}\brak{\frac{1}{2}}$
	\item If $\sin^{-1}x = y$, then
\begin{enumerate}
\begin{multicols}{4}
\item $0 \le y \le \pi$
\item $-\frac{\pi}{2} \le y \le \frac{\pi}{2}$
\item $0 < y < \pi$
\item $-\frac{\pi}{2} < y < \frac{\pi}{2}$
\end{multicols}
\end{enumerate}
	\item $\tan^{-1}\sqrt{3}-\sec^{-1}\brak{-{2}}$ is equal to
\begin{enumerate}
\begin{multicols}{4}
\item $ \pi$
\item $-\frac{\pi}{3}$
\item $\frac{\pi}{3}$
\item $\frac{2\pi}{3}$
\end{multicols}
\end{enumerate}
	\item Show that $\tan^{-1}\brak{\frac{1}{2}}+\tan^{-1}\brak{\frac{2}{11}}=\tan^{-1}\brak{\frac{3}{4}}$.
	\item Express 
		$\tan^{-1}\brak{\frac{\cos x}{1-\sin x}},
-\frac{3\pi}{2} < y < \frac{\pi}{2}$
		in the simplest form.
	\item Write
		$\cot^{-1}\brak{\frac{1}{\sqrt{x^2-1}}},
x > 1$
		in the simplest form.
	\item Find the value of
		$\cos\brak{\sec^{-1}x +\csc^{-1}x},
		\abs{x} \ge 1$.
\end{enumerate}
Prove the following
\begin{enumerate}[label=\thesubsection.\arabic*,ref=\thesubsection.\theenumi,resume*,itemsep=1ex]
	\item 
		$3\sin^{-1}x =\sin^{-1}\brak{3x-4x^3},
		x \in \sbrak{-\frac{1}{2},\frac{1}{2}}$.
	\item 
		$3\cos^{-1}x =\cos^{-1}\brak{4x^3-3x},
		x \in \sbrak{\frac{1}{2},{1}}$.
	\item $\tan^{-1}\brak{\frac{2}{11}}+\tan^{-1}\brak{\frac{7}{24}}=\tan^{-1}\brak{\frac{1}{2}}$.
	\item $2\tan^{-1}\brak{\frac{1}{2}}+\tan^{-1}\brak{\frac{1}{7}}=\tan^{-1}\brak{\frac{31}{17}}$.
\end{enumerate}
Write the following functions in the simplest form
\begin{enumerate}[label=\thesubsection.\arabic*,ref=\thesubsection.\theenumi,resume*,itemsep=1ex]
	\item 
		$\tan^{-1}\brak{\frac{\sqrt{1+x^2}-1}{x}},
x \ne 0$.
	\item 
		$\tan^{-1}\brak{\frac{1}{\sqrt{x^2-1}}},
		\abs{x} > 1$.
	\item 
		$\tan^{-1}\brak{\sqrt{\frac{1-\cos x}{1+\cos x}}},
		0 < {x} < \pi$.
	\item 
		$\tan^{-1}\brak{\frac{\cos x-\sin x}{\cos x+\sin x}},
-\frac{\pi}{4} < x < \frac{3\pi}{4}$.
	\item 
		$\tan^{-1}\brak{\frac{x}{\sqrt{a^2-x^2}}},
		\abs{x} < a$.
	\item 
		$\tan^{-1}\brak{\frac{3a^2x-x^3}{{a^3-3ax^2}}},
		a > 0,
		-\frac{a}{\sqrt{3}} < x < \frac{a}{\sqrt{3}}$
\end{enumerate}
Find the values of each of the following
\begin{enumerate}[label=\thesubsection.\arabic*,ref=\thesubsection.\theenumi,itemsep=1ex]
	\item 
		$\tan^{-1}\sbrak{2\cos \brak{2\sin^{-1}\frac{1}{2}}}$
	\item 
		$\cot\brak{\tan^{-1}a + \cot^{-1}a}$
	\item
		$\tan\frac{1}{2}\sbrak{\sin^{-1}\brak{\frac{2x}{1+x^2}}+\cos^{-1}\brak{\frac{1-y^2}{1+y^2}}},
		\abs{x} < 1, y > 0,  xy < 1$.
\end{enumerate}
Find the values of each of the expressions
\begin{enumerate}[label=\thesubsection.\arabic*,ref=\thesubsection.\theenumi,itemsep=1ex]
	\item 
		$\sin^{-1}\sbrak{\sin\brak{\frac{2\pi}{3}}}$ 
	\item 
		$\tan^{-1}\sbrak{\tan\brak{\frac{3\pi}{4}}}$ 
	\item 
		$\tan\sbrak{\sin^{-1}\brak{\frac{3}{5}}+\cot^{-1}\brak{\frac{3}{2}}}$
	\item 
		$\cos^{-1}\sbrak{\cos \brak{\frac{7\pi}{6}}}$ 
		is equal to 
\begin{enumerate}
\begin{multicols}{4}
	\item 
		$\frac{7\pi}{6}$ 
	\item 
		$\frac{5\pi}{6}$ 
	\item 
		$\frac{\pi}{3}$ 
	\item 
		$\frac{\pi}{6}$ 
\end{multicols}
\end{enumerate}
	\item 
		$\sin\sbrak{\frac{\pi}{3}-\sin^{-1}\brak{-\frac{1}{2}}}$ 
		is equal to 
\begin{enumerate}
\begin{multicols}{4}
	\item 
		$\frac{1}{2}$ 
	\item 
		$\frac{1}{3}$ 
	\item 
		$\frac{1}{4}$ 
	\item 
		$1$ 
\end{multicols}
\end{enumerate}
	\item 
		$\tan^{-1}\sqrt{3}-\cot^{-1}\brak{-\sqrt{3}}$ 
		is equal to 
\begin{enumerate}
\begin{multicols}{4}
	\item 
		$\pi$ 
	\item 
		$-\frac{\pi}{2}$ 
	\item 
		$0$ 
	\item 
		$2\sqrt{3}$ 
\end{multicols}
\end{enumerate}
\item Find the value of $\sin ^{-1}\sin\brak{\frac{3\pi}{5}}$.

\item 	Show that $\sin^{-1}\brak{\frac{3}{5}}-\sin^{-1}\brak{\frac{8}{17}}=\cos^{-1}\brak{\frac{84}{85}}$.
\item 	Show that $\sin^{-1}\brak{\frac{12}{13}}+\cos^{-1}\brak{\frac{4}{5}}+\tan^{-1}\brak{\frac{63}{16}}=\pi$.
	\item Simplify
		$\tan^{-1}\brak{\frac{a\cos x-b\sin x}{b\cos x+a\sin x}}$, if $
\frac{a}{b}\tan x > -1$.
\end{enumerate}
Find the value of the following
\begin{enumerate}[label=\thesubsection.\arabic*,ref=\thesubsection.\theenumi,resume*,itemsep=1ex]
\item $\cos^{-1}\cos\brak{\frac{13\pi}{6}}$.
\item $\tan^{-1}\tan\brak{\frac{7\pi}{6}}$.
\end{enumerate}
Prove that
\begin{enumerate}[label=\thesubsection.\arabic*,ref=\thesubsection.\theenumi,resume*,itemsep=1ex]
	\item $2\sin^{-1}\brak{\frac{3}{5}} = \tan^{-1}\brak{\frac{24}{7}}$.
\item $\sin^{-1}\brak{\frac{8}{17}} +\sin^{-1}\brak{\frac{3}{5}} = \tan^{-1}\brak{\frac{77}{36}}$.
\item $\cos^{-1}\brak{\frac{4}{5}} +\cos^{-1}\brak{\frac{12}{13}} = \cos^{-1}\brak{\frac{33}{65}}$.
\item $\cos^{-1}\brak{\frac{12}{13}} +\sin^{-1}\brak{\frac{3}{5}} = \sin^{-1}\brak{\frac{56}{65}}$.
\item $\tan^{-1}\brak{\frac{63}{16}} =\sin^{-1}\brak{\frac{5}{13}} + \cos^{-1}\brak{\frac{3}{5}}$.
\item $\tan^{-1}\brak{\frac{1}{5}} +\tan^{-1}\brak{\frac{1}{7}} + \tan^{-1}\brak{\frac{1}{3}}+ \tan^{-1}\brak{\frac{1}{8}} = \frac{\pi}{4}$.
\end{enumerate}
Prove that
\begin{enumerate}[label=\thesubsection.\arabic*,ref=\thesubsection.\theenumi,resume*,itemsep=1ex]
	\item 
		$\tan^{-1}\sqrt{x}=\frac{1}{2}\cos^{-1}\brak{\frac{1-x}{1+x}}, x \in \sbrak{0,1}$.
	\item 
		$\cot^{-1}\brak{\frac{\sqrt{1+\sin x}+\sqrt{1-\sin x}}{{\sqrt{1+\sin x}-\sqrt{1-\sin x}}}}=\frac{x}{2}, x \in \brak{0,\frac{\pi}{4}}$.
	\item 
		$\tan^{-1}\brak{\frac{\sqrt{1+ x}-\sqrt{1- x}}{{\sqrt{1+ x}+\sqrt{1- x}}}}=\frac{\pi}{4}-\frac{1}{2}\cos^{-1}x, -\frac{1}{\sqrt{2}} \le x \le 1$.
	\item 	$\frac{9\pi}{8}-\frac{9}{4}\sin^{-1}\brak{\frac{1}{3}}=\frac{9}{4}\sin^{-1}\brak{\frac{2\sqrt{2}}{3}}$.
\end{enumerate}
